examples/cost/flat_sumProofScript.sml
@@ -1,0 +1,690 @@
+(*
+  Prove of sum space consumption
+*)
+
+open preamble basis compilationLib;
+open backendProofTheory backendPropsTheory
+open costLib costPropsTheory flat_size_ofPropsTheory
+open dataSemTheory data_monadTheory dataLangTheory;
+open x64_configProofTheory;
+open sumProgTheory;
+
+val _ = temp_delsimps ["NORMEQ_CONV"]
+
+val _ = new_theory "flat_sumProof"
+
+val _ = ParseExtras.temp_tight_equality ()
+
+Overload monad_unitbind[local] = ``data_monad$bind``
+Overload return[local] = ``data_monad$return``
+val _ = monadsyntax.temp_add_monadsyntax()
+
+val sum_x64_conf = (rand o rator o lhs o concl) sum_thm
+
+val _ = install_naming_overloads "sumProg";
+val _ = write_to_file sum_data_prog_def;
+
+val fields = TypeBase.fields_of “:('c,'ffi) dataSem$state”;
+
+Overload state_refs_fupd = (fields |> assoc "refs" |> #fupd);
+Overload state_locals_fupd = (fields |> assoc "locals" |> #fupd);
+Overload state_stack_max_fupd = (fields |> assoc "stack_max" |> #fupd);
+Overload state_safe_for_space_fupd = (fields |> assoc "safe_for_space" |> #fupd);
+Overload state_peak_heap_length_fupd = (fields |> assoc "peak_heap_length" |> #fupd);
+
+val foldl_body = ``lookup_List_foldl (fromAList sum_data_prog)``
+           |> (REWRITE_CONV [sum_data_code_def] THENC EVAL)
+           |> concl |> rhs |> rand |> rand
+
+Definition foldl_body_def:
+  foldl_body = ^foldl_body
+End
+
+val Int_plus_clos_body = ``lookup_Int_+_clos (fromAList sum_data_prog)``
+           |> (REWRITE_CONV [sum_data_code_def] THENC EVAL)
+           |> concl |> rhs |> rand |> rand
+
+Definition Int_plus_clos_body_def:
+  Int_plus_clos_body = ^Int_plus_clos_body
+End
+
+val Int_plus_body = ``lookup_Int_+ (fromAList sum_data_prog)``
+           |> (REWRITE_CONV [sum_data_code_def] THENC EVAL)
+           |> concl |> rhs |> rand |> rand
+
+Definition Int_plus_body_def:
+  Int_plus_body = ^Int_plus_body
+End
+
+(* The maximum amount of heap space that will be consumed by the accumulator (e) when
+   adding all number in the list
+ *)
+Definition sum_heap_size_def:
+  sum_heap_size s e []      = 0 ∧
+  sum_heap_size s e (x::xs) = MAX (space_consumed s Add [Number e; Number x])
+                                  (sum_heap_size s (e+x) xs)
+End
+
+(* The maximum amount of stack space that will be consumed by the accumulator (e) when
+   adding all number in the list
+ *)
+Definition sum_stack_size_def:
+  sum_stack_size sfs lims e []      = SOME 0 ∧
+  sum_stack_size sfs lims e (x::xs) = OPTION_MAP2 MAX (stack_consumed sfs lims (Add) [Number e; Number x])
+                                                      (sum_stack_size sfs lims (e+x) xs)
+End
+
+(* Turns a ‘v’ value into a ‘int list’; returns NONE if something goes wrong *)
+Definition repint_to_list_def:
+  repint_to_list (Block _ _ [Number i; rest]) = OPTION_MAP (CONS i) (repint_to_list rest) ∧
+  repint_to_list (Block _ 0 []) = SOME [] ∧
+  repint_to_list _ = NONE
+End
+
+(* The only part of the state that affects the list's heap usage is ‘limits’ *)
+Theorem sum_heap_size_eq:
+  ∀s1 s2 l e.
+   s1.limits = s2.limits ⇒ sum_heap_size s2 e l = sum_heap_size s1 e l
+Proof
+  ntac 2 strip_tac
+  \\ Induct \\ rw [sum_heap_size_def,space_consumed_def]
+QED
+
+(* The size of the biggest number in the list *)
+Definition bigest_num_size_def:
+  bigest_num_size lims [] = 0
+∧ bigest_num_size lims (x::xs) =
+    MAX (FST (size_of lims [Number x] LN LN))
+             (bigest_num_size lims xs)
+End
+
+(* How big the accumulator will ever get *)
+Definition bigest_acc_size_def:
+  bigest_acc_size lims acc [] = 0
+∧ bigest_acc_size lims acc (x::xs) =
+    (FST (size_of lims [Number (acc+x)] LN LN) - FST (size_of lims [Number acc] LN LN)) +
+    (bigest_acc_size lims (acc+x) xs)
+End
+
+Theorem Int_plus_evaluate:
+  ∀s i1 i2 sstack smax ssum.
+    (* Sizes *)
+    size_of_stack s.stack = SOME sstack ∧
+    s.locals_size = SOME 4 ∧
+    s.stack_max = SOME smax ∧
+    (* Arguments *)
+    s.locals = fromList [Number i2; Number i1] ∧
+    (* Stack frames *)
+    s.stack_frame_sizes = sum_config.word_conf.stack_frame_size ∧
+    (* Limits *)
+    stack_consumed s.stack_frame_sizes s.limits Add [Number i1; Number i2] = SOME ssum ∧
+    smax < s.limits.stack_limit ∧
+    sstack + 4 + ssum < s.limits.stack_limit ∧
+    size_of_heap s + space_consumed s Add [Number i1; Number i2] ≤ s.limits.heap_limit ∧
+    lim_safe s.limits Add [Number i1; Number i2] ∧
+    (* Code *)
+    (* Invariants *)
+    s.safe_for_space ∧
+    s.limits.arch_64_bit
+    (* s.tstamps = SOME ts ∧ *)
+    (* 1 < s.limits.length_limit *)
+    ⇒
+    ∃pkheap0.
+     evaluate (Int_plus_body,s) =
+       (SOME (Rval (Number (i1+i2))), s with <| locals := LN;
+                                                locals_size := SOME 0;
+                                                space := 0;
+                                                stack_max := SOME (MAX smax (sstack + 4 + ssum));
+                                                peak_heap_length := pkheap0
+                            |>)
+Proof
+  rw[Int_plus_body_def]
+  \\ REWRITE_TAC[to_shallow_thm,to_shallow_def]
+  \\ qpat_x_assum ‘s.locals = _’ (assume_tac o EVAL_RULE)
+  \\ qmatch_goalsub_abbrev_tac `bind _ rest_ass _`
+  \\ simp [bind_def,assign_def,cut_state_opt_def,
+           cut_state_def,cut_env_def]
+  \\ eval_goalsub_tac ``dataSem$get_vars    _ _`` \\ simp []
+  \\ simp[do_app_def,do_app_aux_def,do_space_def,
+          op_space_reset_def,set_var_def,do_stack_def]
+  \\ qunabbrev_tac ‘rest_ass’
+  \\ simp [return_def,flush_state_def,state_component_equality]
+  \\ fs [size_of_stack_def] \\ rfs []
+  \\ (conj_tac
+      >- (eval_goalsub_tac ``state_locals_fupd _ _``
+          \\ qmatch_goalsub_abbrev_tac ‘size_of_heap ss’
+          \\ ‘ss = s’ suffices_by rw []
+          \\ UNABBREV_ALL_TAC \\ rw [state_component_equality])
+      \\ EVAL_TAC)
+QED
+
+(* Every addition performed stays within the length_limit *)
+Definition foldadd_limit_ok_def:
+  foldadd_limit_ok lims acc il =
+  ((*(small_num lims.arch_64_bit acc ∨
+   bignum_size lims.arch_64_bit acc ≤ 2 ** lims.length_limit) ∧  *)
+   (∀n.
+      n < LENGTH il ⇒
+      let i1 = acc + FOLDR $+ 0 (TAKE n il);
+          i2 = EL n il
+      in
+        lim_safe lims Add [Number i1; Number i2]))
+End
+
+Theorem foldadd_limits_ok_step:
+  foldadd_limit_ok lims acc (n::l) ⇒
+  foldadd_limit_ok lims (acc + n) l
+Proof
+  rw[foldadd_limit_ok_def] >>
+  rename1 ‘m < LENGTH l’ >>
+  first_x_assum(qspec_then ‘SUC m’ mp_tac) >>
+  rw[] >>
+  fs[AC integerTheory.INT_ADD_SYM integerTheory.INT_ADD_ASSOC]
+QED
+
+Theorem le_right_add:
+  a ≤ b ⇒ a ≤ b + (c:num)
+Proof
+  intLib.ARITH_TAC
+QED
+
+Theorem bignum_digits_LESS_EQ:
+  ∀b m n. n ≤ m ⇒ bignum_digits b n ≤ bignum_digits b m
+Proof
+  ho_match_mp_tac bignum_digits_ind \\ rw []
+  \\ once_rewrite_tac [bignum_digits_def] \\ rw [] \\ fs []
+  \\ first_x_assum match_mp_tac
+  \\ fs [X_LE_DIV]
+  \\ match_mp_tac LESS_EQ_TRANS
+  \\ once_rewrite_tac [CONJ_COMM]
+  \\ asm_exists_tac \\ fs []
+  THENL [‘0 < 18446744073709551616n’ by fs [], ‘0 < 4294967296n’ by fs []]
+  \\ drule DIVISION
+  \\ disch_then (fn th => CONV_TAC (RAND_CONV (ONCE_REWRITE_CONV [th])))
+  \\ fs []
+QED
+
+Theorem bignum_digits_LESS_EQ_ADD:
+  k ≤ bignum_digits f (n + n') ⇒
+  k ≤ SUC (bignum_digits f n + bignum_digits f n')
+Proof
+  rw [] \\ match_mp_tac LESS_EQ_TRANS
+  \\ asm_exists_tac \\ fs []
+  \\ pop_assum kall_tac
+  \\ completeInduct_on ‘n+n'’
+  \\ rw [] \\ fs [PULL_FORALL]
+  \\ once_rewrite_tac [bignum_digits_def] \\ rw [] \\ fs []
+  \\ rewrite_tac [DECIDE “2 = SUC (SUC 0n) ∧ 1 = SUC 0”,ADD_CLAUSES,LESS_EQ_MONO]
+  \\ simp [Once bignum_digits_def]
+  \\ rw []
+  \\ rewrite_tac [DECIDE “2 = SUC (SUC 0n) ∧ 1 = SUC 0”,ADD_CLAUSES,LESS_EQ_MONO]
+  \\ qmatch_goalsub_abbrev_tac ‘_ DIV k’
+  \\ first_x_assum (qspecl_then [‘n DIV k’,‘n' DIV k’] mp_tac)
+  \\ (impl_tac THEN1
+   (match_mp_tac (DECIDE “m < n ∧ m' < n' ⇒ m + m' < n + n':num”)
+    \\ fs [Abbr‘k’,DIV_LT_X]))
+  \\ rw [] \\ match_mp_tac LESS_EQ_TRANS
+  \\ once_rewrite_tac [CONJ_COMM]
+  \\ asm_exists_tac \\ fs []
+  \\ match_mp_tac bignum_digits_LESS_EQ
+  \\ ‘0 < k’ by fs [Abbr‘k’]
+  \\ fs [DIV_LE_X,DIV_LT_X]
+  \\ fs [LEFT_ADD_DISTRIB]
+  \\ drule DIVISION
+  \\ disch_then (fn th =>
+       strip_assume_tac (Q.SPEC ‘n’ th) THEN
+       strip_assume_tac (Q.SPEC ‘n'’ th))
+  \\ unabbrev_all_tac
+  \\ full_simp_tac bool_ss [EVAL “18446744073709551616n²”]
+  \\ full_simp_tac bool_ss [EVAL “4294967296n²”]
+  \\ decide_tac
+QED
+
+Theorem bignum_size_plus:
+  bignum_size f (a+b) ≤ bignum_size f a + bignum_size f b
+Proof
+  fs [bignum_size_def]
+  \\ Cases_on ‘a’ \\ fs [] \\ Cases_on ‘b’ \\ fs []
+  \\ fs [integerRingTheory.int_calculate] \\ rw []
+  \\ rewrite_tac [DECIDE “2 = SUC (SUC 0n) ∧ 1 = SUC 0”,ADD_CLAUSES,LESS_EQ_MONO]
+  \\ match_mp_tac bignum_digits_LESS_EQ_ADD \\ fs []
+  \\ match_mp_tac bignum_digits_LESS_EQ \\ fs []
+QED
+
+Theorem foldl_evaluate:
+  ∀vl il s acc ts_f tag_f sstack lsize ssum smax.
+    (* Sizes *)
+    size_of_stack s.stack = SOME sstack ∧
+    s.locals_size = SOME lsize ∧
+    lookup_List_foldl s.stack_frame_sizes = SOME lsize ∧
+    s.stack_max = SOME smax ∧
+    s.space = 0 ∧
+    (* Arguments *)
+    s.locals = fromList [vl ; Number acc; Block ts_f tag_f [CodePtr_Int_+_clos;Number 1]] ∧
+    repint_to_list vl = SOME il ∧
+    (* Stack frames *)
+    s.stack_frame_sizes = sum_config.word_conf.stack_frame_size ∧
+    sum_stack_size s.stack_frame_sizes s.limits acc il = SOME ssum ∧
+    (* Limits *)
+    smax < s.limits.stack_limit ∧
+    sstack + lsize + ssum + 4 < s.limits.stack_limit ∧
+    flat_size_of_heap s + bigest_acc_size s.limits acc il +
+    bigest_num_size s.limits il + sum_heap_size s acc il ≤ s.limits.heap_limit ∧
+    foldadd_limit_ok s.limits acc il ∧
+    (* Code *)
+    lookup_List_foldl s.code = SOME (3,foldl_body) ∧
+    lookup_Int_+_clos s.code = SOME (3,Int_plus_clos_body) ∧
+    lookup_Int_+ s.code      = SOME (2,Int_plus_body) ∧
+    (* Invariants *)
+    size_inv s ∧ (* Needed, since there is no heap allocation in the function *)
+    s.safe_for_space ∧
+    s.limits.arch_64_bit ∧
+    1 < s.limits.length_limit
+    ⇒
+    ∃res lcls0 lsz0 smax0 clk0 ts0 pkheap0 stk.
+     evaluate (foldl_body,s) =
+       (SOME res, s with <| locals := lcls0;
+                            locals_size := lsz0;
+                            stack_max := SOME smax0;
+                            clock := clk0;
+                            tstamps := ts0;
+                            peak_heap_length := pkheap0;
+                            stack := stk;
+                            space := 0
+                            |>) ∧
+     clk0 ≤ s.clock ∧
+     (res = (Rerr(Rabort Rtimeout_error)) ∨
+      ∃sumi. res = Rval (Number sumi) ∧ (stk = s.stack) ∧
+             smax0 = MAX smax (lsize + sstack + (if il = [] then 0 else 4) + ssum))
+Proof
+let
+  val code_lookup   = mk_code_lookup
+                        `fromAList sum_data_prog`
+                         sum_data_code_def
+  val frame_lookup   = mk_frame_lookup
+                        `sum_config.word_conf.stack_frame_size`
+                         sum_config_def
+  val strip_assign  = mk_strip_assign code_lookup frame_lookup
+  val open_call     = mk_open_call code_lookup frame_lookup
+  val make_call     = mk_make_call open_call
+  val strip_call    = mk_strip_call open_call
+  val open_tailcall = mk_open_tailcall code_lookup frame_lookup
+  val make_tailcall = mk_make_tailcall open_tailcall
+  fun max_is t =
+    qmatch_goalsub_abbrev_tac `state_stack_max_fupd (K max0) _` >>
+    subgoal ‘max0 = SOME (^(Term t))’
+    THENL
+    [(Q.UNABBREV_TAC ‘max0’ \\ fs [small_num_def,size_of_stack_def]),
+    ASM_REWRITE_TAC [] \\ ntac 2 (pop_assum kall_tac)]
+in
+  ho_match_mp_tac repint_to_list_ind
+  \\ rw[foldl_body_def,Int_plus_body_def,Int_plus_clos_body_def,repint_to_list_def]
+  \\ REWRITE_TAC[to_shallow_thm,to_shallow_def]
+  \\ qpat_x_assum ‘s.locals = _’ (assume_tac o EVAL_RULE)
+  >~ [‘Block v2 0 []’]
+  >- (strip_assign \\ make_if
+     \\ rw [state_component_equality]
+     \\ fs [repint_to_list_def] \\ rveq
+     \\ fs [sum_stack_size_def] \\ rveq
+     \\ fs [])
+  \\ strip_assign
+  \\ make_if
+  \\ rename1`Block ts_vl tag_vl [Number i; vl]`
+  \\ ntac 4 strip_assign
+  \\ ONCE_REWRITE_TAC [bind_def]
+  \\ make_if
+  \\ strip_assign
+  \\ max_is ‘MAX smax (lsize + sstack)’
+  >- fs [MAX_DEF]
+  \\ strip_call
+  \\ open_tailcall
+  \\ max_is ‘MAX smax (lsize + sstack + 4)’
+  >- fs [MAX_DEF]
+  \\ qmatch_goalsub_abbrev_tac `state_safe_for_space_fupd (K safe)  _`
+  \\ ‘safe’ by
+     (qunabbrev_tac ‘safe’ \\ fs [size_of_stack_def,GREATER_DEF] \\ EVAL_TAC)
+  \\ simp [] \\ ntac 2 (pop_assum kall_tac)
+  \\ fs [repint_to_list_def] \\ rveq
+  \\ fs [sum_stack_size_def]
+  \\ qmatch_goalsub_abbrev_tac ‘bind _ _ s'’
+  \\ qspecl_then [‘s'’,‘acc’,‘i’] mp_tac Int_plus_evaluate
+  \\ disch_then (qspecl_then [‘THE (size_of_stack s'.stack)’,
+                              ‘THE (s'.stack_max)’,
+                              ‘x1’] mp_tac)
+  \\ impl_tac
+  >- (qunabbrev_tac ‘s'’ \\ rw []
+     >- fs [size_of_stack_def,size_of_stack_frame_def]
+     >- EVAL_TAC
+     >- rfs []
+     >- (Cases_on ‘x1 ≤ x2’ \\ fs [MAX_DEF,size_of_stack_frame_def,size_of_stack_def])
+     >- (fs[space_consumed_def,sum_heap_size_def]
+         \\ qmatch_goalsub_abbrev_tac ‘size_of_heap s0 + s_consumed’
+         \\ ‘size_inv s0’ by
+           (qpat_x_assum ‘size_inv _’ mp_tac
+            \\ gs[Abbr‘s0’,size_inv_def,all_blocks_inv_def,stack_to_vs_def]
+            \\ eval_goalsub_tac ``sptree$toList _``
+            \\ ONCE_REWRITE_TAC[GSYM APPEND_ASSOC]
+            \\ qmatch_goalsub_abbrev_tac ‘_ ++ rest’
+            \\ eval_goalsub_tac ``sptree$toList _``
+            \\ rw[all_blocks_roots_inv_def]
+            >- (gs[all_blocks_blocks_inv_def]
+                \\ qmatch_asmsub_abbrev_tac ‘Block ts_vl _ ll’
+                \\ first_x_assum (qspecl_then [‘ts_vl’,‘tag_vl’,‘ll’] mp_tac)
+                \\ impl_tac >- (first_x_assum (irule_at Any) \\ simp[Abbr‘ll’])
+                \\ simp[Abbr‘ll’]
+                \\ qpat_x_assum ‘MEM _ _’ mp_tac
+                \\ eval_goalsub_tac “MEM (Block _ _ _) _”
+                \\ simp[IN_DEF] \\ rw[]
+                >- (first_x_assum (irule_at Any) \\ simp[])
+                \\ pop_assum mp_tac
+                \\ rw[all_blocks_roots_inv_def]
+                \\ first_x_assum irule
+                \\ simp[])
+          >- (first_x_assum (irule_at Any) \\ simp[]))
+         \\ drule size_of_heap_eq_flat_size_of_heap
+         \\ pop_assum (simp o single)
+         \\ ‘flat_size_of_heap s0 ≤ flat_size_of_heap s + bigest_num_size s.limits (i::z)’ suffices_by
+             (Cases_on ‘s_consumed ≤ sum_heap_size s (acc + i) z’ \\ fs [MAX_DEF])
+         \\ qunabbrev_tac ‘s0’
+         \\ simp [flat_size_of_heap_def,stack_to_vs_def,
+                  toList_def,toListA_def,extract_stack_def]
+         \\ qmatch_goalsub_abbrev_tac ‘Number acc::rest_v’
+         \\ simp[flat_size_of_def]
+         \\ qmatch_goalsub_abbrev_tac ‘a + c ≤ b + d’
+         \\ ‘c ≤ d ∧ a ≤ b’ suffices_by simp[]
+         \\ conj_tac
+         >- (UNABBREV_ALL_TAC
+             \\ simp[flat_measure_def]
+             \\ Cases_on ‘vl’ \\ gs[repint_to_list_def,flat_measure_def]
+             \\ qmatch_goalsub_abbrev_tac ‘a + b ≤ c + _’
+             \\ ‘b ≤ c’ suffices_by simp[]
+             \\ rw[Abbr‘b’,Abbr‘c’,bigest_num_size_def,bignum_size_def,size_of_def])
+         \\ simp[Abbr‘a’,Abbr‘b’]
+         \\ irule SUM_IMAGE_SUBSET_LE
+         \\ conj_tac >- simp[FINITE_reachable_v,FINITE_to_addrs]
+         \\ simp[to_addrs_def] \\ simp[Once to_addrs_cons]
+         \\ rw[reachable_v_def,SUBSET_DEF,FUN_EQ_THM]
+         >- (first_x_assum (irule_at Any) \\ simp[])
+         >- (qexists_tac ‘BlockAddr ts_vl’ \\ simp[]
+             \\ irule ((snd o EQ_IMP_RULE o SPEC_ALL) RTC_CASES1)
+             \\ disj2_tac \\ first_x_assum (irule_at Any)
+             \\ simp[next_def,block_to_addrs_def,IN_DEF]
+             \\ gs[size_inv_def,all_blocks_inv_def,all_blocks_roots_inv_def]
+             \\ first_x_assum (qspecl_then [‘ts_vl’,‘tag_vl’,‘[Number i; vl]’] mp_tac)
+             \\ impl_tac
+             >- (simp[stack_to_vs_def,toListA_def,toList_def])
+             \\ gs[to_addrs_def,IN_DEF])
+         >- (first_x_assum (irule_at Any) \\ simp[]))
+     \\ qhdtm_x_assum ‘foldadd_limit_ok’ mp_tac
+     \\ simp[foldadd_limit_ok_def]
+     \\ disch_then(qspec_then ‘0’ mp_tac) \\ simp[])
+  \\ REWRITE_TAC [Int_plus_body_def,to_shallow_thm,to_shallow_def]
+  \\ rw [] \\ simp []
+  \\ qunabbrev_tac ‘s'’
+  \\ simp [pop_env_def,set_var_def]
+  \\ qunabbrev_tac ‘rest_call’
+  \\ eval_goalsub_tac ``state_locals_fupd _ _``
+  \\ max_is ‘MAX smax (lsize + sstack + x1 + 4)’
+  >- fs [MAX_DEF]
+  \\ simp [move_def,lookup_def,set_var_def,lookup_insert]
+  \\ IF_CASES_TAC >- rw [state_component_equality]
+  \\ qmatch_goalsub_abbrev_tac ‘to_shallow _ s'’
+  \\ first_x_assum (qspec_then ‘s'’ mp_tac)
+  \\ rveq \\ fs []
+  \\ disch_then (qspecl_then [‘acc + i’,‘ts_f’,‘tag_f’] mp_tac)
+  \\ disch_then (qspecl_then [‘THE (size_of_stack s'.stack)’,‘THE s'.locals_size’] mp_tac)
+  \\ disch_then (qspecl_then [‘x2’,‘THE s'.stack_max’] mp_tac)
+  \\ impl_tac
+  >- (qunabbrev_tac ‘s'’
+     \\ rw [frame_lookup,foldl_body_def,Int_plus_body_def,Int_plus_clos_body_def]
+     \\ rfs []
+     >- (Cases_on ‘x1 ≤ x2’ \\ fs [MAX_DEF])
+     >- (rfs [frame_lookup] \\ rveq \\ fs []
+         \\ Cases_on ‘x1 ≤ x2’ \\ fs [MAX_DEF])
+     >- (qmatch_goalsub_abbrev_tac ‘sum_heap_size s'’
+         \\ qspecl_then [‘s’,‘s'’,‘z’,‘acc + i’] mp_tac sum_heap_size_eq
+         \\ impl_tac >- (UNABBREV_ALL_TAC \\ rw []) \\ rw []
+         \\ pop_assum kall_tac
+         \\ qmatch_asmsub_abbrev_tac ‘flat_size_of_heap s  + (cc + (bb + ss))’
+         \\ qmatch_goalsub_abbrev_tac ‘flat_size_of_heap s' + (cc' + (bb' + ss'))’
+         \\ `ss' ≤ ss` by
+            (unabbrev_all_tac \\ simp[sum_heap_size_def])
+         \\ ‘cc' ≤ cc’ by
+            (unabbrev_all_tac \\ simp[bigest_num_size_def])
+         \\ `flat_size_of_heap s' + bb' ≤ flat_size_of_heap s + bb` suffices_by fs[]
+         \\ pop_assum kall_tac \\ pop_assum kall_tac
+         \\ qunabbrev_tac ‘s'’
+         \\ eval_goalsub_tac ``state_locals_fupd _ _``
+         \\ simp [flat_size_of_heap_def,stack_to_vs_def,
+                  toList_def,toListA_def,extract_stack_def]
+         \\ qmatch_goalsub_abbrev_tac ‘Number acc::rest_v’
+         \\ simp[flat_size_of_def]
+         \\ ONCE_REWRITE_TAC [ADD_ASSOC]
+         \\ ONCE_REWRITE_TAC [ADD_ASSOC]
+         \\ qmatch_goalsub_abbrev_tac ‘_ + r + a + b ≤ _ + _ + c + d’
+         \\ ‘bb' + r + b ≤ bb + r + d ∧ a ≤ c’ suffices_by simp[]
+         \\ conj_tac
+         >- (UNABBREV_ALL_TAC
+             \\ simp[flat_measure_def]
+             \\ Cases_on ‘vl’ \\ gs[repint_to_list_def,flat_measure_def]
+             \\ simp [size_of_def,sum_heap_size_def,
+                      space_consumed_def,bigest_acc_size_def]
+             \\ rw [])
+         \\ simp[Abbr‘a’,Abbr‘c’]
+         \\ irule SUM_IMAGE_SUBSET_LE
+         \\ conj_tac >- simp[FINITE_to_addrs,FINITE_reachable_v]
+         \\ simp[to_addrs_def] \\ simp[Once to_addrs_cons]
+         \\ rw[reachable_v_def,SUBSET_DEF,FUN_EQ_THM]
+         >- (first_x_assum (irule_at Any) \\ simp[])
+         >- (qexists_tac ‘BlockAddr ts_vl’ \\ simp[]
+             \\ irule ((snd o EQ_IMP_RULE o SPEC_ALL) RTC_CASES1)
+             \\ disj2_tac \\ first_x_assum (irule_at Any)
+             \\ simp[next_def,block_to_addrs_def,IN_DEF]
+             \\ gs[size_inv_def,all_blocks_inv_def,all_blocks_roots_inv_def]
+             \\ first_x_assum (qspecl_then [‘ts_vl’,‘tag_vl’,‘[Number i; vl]’] mp_tac)
+             \\ impl_tac
+             >- (simp[stack_to_vs_def,toListA_def,toList_def])
+             \\ gs[to_addrs_def,IN_DEF])
+         >- (first_x_assum (irule_at Any) \\ gs[to_addrs_def] \\ simp[]))
+      >- (imp_res_tac foldadd_limits_ok_step)
+      >- (qpat_x_assum ‘size_inv _’ mp_tac
+          \\ gs[size_inv_def,all_blocks_inv_def,stack_to_vs_def]
+          \\ eval_goalsub_tac ``sptree$toList _``
+          \\ ONCE_REWRITE_TAC[GSYM APPEND_ASSOC]
+          \\ qmatch_goalsub_abbrev_tac ‘_ ++ rest’
+          \\ eval_goalsub_tac ``sptree$toList _``
+          \\ rw[all_blocks_roots_inv_def]
+          >- (first_x_assum (irule_at Any) \\ simp[])
+          >- (gs[all_blocks_blocks_inv_def]
+              \\ qmatch_asmsub_abbrev_tac ‘Block ts_vl _ ll’
+              \\ first_x_assum (qspecl_then [‘ts_vl’,‘tag_vl’,‘ll’] mp_tac)
+              \\ impl_tac >- (first_x_assum (irule_at Any) \\ simp[Abbr‘ll’])
+              \\ rw[all_blocks_roots_inv_def]
+              \\ first_x_assum irule
+              \\ simp[Abbr‘ll’])
+          >- (first_x_assum (irule_at Any) \\ simp[]))
+      >- (fs [GREATER_DEF] \\ Cases_on ‘x1 ≤ x2’ \\ fs [MAX_DEF] \\ EVAL_TAC))
+  \\ REWRITE_TAC[to_shallow_thm,to_shallow_def,foldl_body_def]
+  \\ rw [] \\ qunabbrev_tac ‘s'’ \\ simp []
+  \\ simp [state_component_equality,GREATER_DEF] \\ fs []
+  >- (Cases_on ‘x1 ≤ x2’ \\ fs [MAX_DEF] \\ EVAL_TAC)
+  >- (reverse conj_tac
+     >- (Cases_on ‘x1 ≤ x2’ \\ fs [MAX_DEF] \\ EVAL_TAC)
+     \\ rveq \\ fs [sum_stack_size_def] \\ rveq
+     \\ rw [MAX_DEF])
+  >- (Cases_on ‘x1 ≤ x2’ \\ fs [MAX_DEF] \\ EVAL_TAC)
+  \\ rw [MAX_DEF]
+  \\ Cases_on ‘x1 ≤ x2’ \\ fs [MAX_DEF] \\ EVAL_TAC
+end
+QED
+
+Theorem data_safe_sum:
+   ∀ffi.
+  backend_config_ok ^sum_x64_conf
+  ⇒ is_safe_for_space ffi
+       sum_x64_conf
+       sum_prog
+       (* (s_size,h_size) *)
+       (56,112)
+Proof
+let
+  val code_lookup   = mk_code_lookup
+                        `fromAList sum_data_prog`
+                         sum_data_code_def
+  val frame_lookup   = mk_frame_lookup
+                        `sum_config.word_conf.stack_frame_size`
+                         sum_config_def
+  val strip_assign  = mk_strip_assign code_lookup frame_lookup
+  val open_call     = mk_open_call code_lookup frame_lookup
+  val make_call     = mk_make_call open_call
+  val strip_call    = mk_strip_call open_call
+  val open_tailcall = mk_open_tailcall code_lookup frame_lookup
+  val make_tailcall = mk_make_tailcall open_tailcall
+in
+ REWRITE_TAC [sum_prog_def,sum_x64_conf_def]
+ \\ strip_tac \\ strip_tac
+ \\ irule IMP_is_safe_for_space_alt \\ fs []
+ \\ conj_tac >- EVAL_TAC
+ \\ assume_tac sum_thm
+ \\ asm_exists_tac \\ fs []
+ \\ assume_tac sum_to_data_updated_thm
+ \\ fs [data_lang_safe_for_space_def]
+ \\ strip_tac
+ \\ qmatch_goalsub_abbrev_tac `_ v0`
+ \\ `data_safe v0` suffices_by
+    (Cases_on `v0` \\ fs [data_safe_def])
+ \\ UNABBREV_ALL_TAC
+ \\ qmatch_goalsub_abbrev_tac `is_64_bits c0`
+ \\ `is_64_bits c0` by (UNABBREV_ALL_TAC \\ EVAL_TAC)
+ \\ fs []
+ \\ rpt (pop_assum kall_tac)
+ (* start data_safe proof *)
+ \\ REWRITE_TAC [ to_shallow_thm
+                , to_shallow_def
+                , initial_state_def
+                , bvl_to_bviTheory.InitGlobals_location_eq]
+ (* Make first call *)
+ \\ make_tailcall
+ (* Bootcode *)
+ \\ ntac 7 strip_assign
+ \\ ho_match_mp_tac data_safe_bind_return
+ (* Yet another call *)
+ \\ make_call
+ \\ strip_call
+ \\ ntac 9 strip_assign
+ \\ make_if
+ \\ UNABBREV_ALL_TAC
+ \\ strip_makespace
+ \\ ntac 47 strip_assign
+ \\ make_tailcall
+ \\ ntac 4
+    (strip_call
+    \\ ntac 9 strip_assign
+    \\ make_if
+     \\ UNABBREV_ALL_TAC)
+  \\ ntac 6 strip_assign
+  \\ ntac 4
+     (open_tailcall
+     \\ ntac 4 strip_assign
+     \\ make_if
+     \\ ntac 2 strip_assign)
+  \\ open_tailcall
+  \\ ntac 4 strip_assign
+  \\ make_if
+  \\ ASM_REWRITE_TAC [code_lookup,frame_lookup]
+  \\ simp []
+  \\ IF_CASES_TAC >- (simp [data_safe_def,size_of_def,frame_lookup] \\ EVAL_TAC)
+  \\ REWRITE_TAC [to_shallow_def]
+  \\ strip_makespace
+  \\ ntac 3 strip_assign
+  \\ make_tailcall
+  \\ ntac 3
+     (strip_makespace
+     \\ ntac 4 strip_assign
+     \\ make_tailcall)
+  \\ ntac 31 strip_assign
+  \\ strip_makespace
+  \\ ntac 9 strip_assign
+  \\ qmatch_goalsub_abbrev_tac `f (state_locals_fupd _ _)`
+  \\ qmatch_goalsub_abbrev_tac `f s`
+  \\ irule data_safe_res
+  \\ conj_tac >- (Cases \\ simp [] \\ IF_CASES_TAC \\ simp [])
+  \\ UNABBREV_ALL_TAC
+  \\ strip_call
+  \\ ntac 2 strip_assign
+  \\ open_tailcall
+  \\ qmatch_goalsub_abbrev_tac ‘(bind _ _) st’
+  \\ qabbrev_tac ‘vl = THE(sptree$lookup (0:num) st.locals)’
+  \\ qabbrev_tac ‘il = THE(repint_to_list vl)’
+  \\ qabbrev_tac ‘ssum = THE(sum_stack_size st.stack_frame_sizes st.limits 0 il)’
+  \\ qspecl_then [‘vl’,‘il’,‘st’,‘0’,‘1’,‘30’] mp_tac foldl_evaluate
+  \\ simp[LEFT_FORALL_IMP_THM]
+  \\ disch_then(mp_tac o CONV_RULE(RESORT_FORALL_CONV List.rev))
+  \\ disch_then(qspecl_then [‘THE(st.stack_max)’,‘ssum’,
+                             ‘THE(st.locals_size)’,
+                             ‘THE(size_of_stack st.stack)’] mp_tac)
+  \\ simp[LEFT_FORALL_IMP_THM]
+  \\ impl_tac
+  (* Prove that the preconditions of foldl_evaluate are satisfied *)
+  >- (‘size_inv st’ by
+       (simp[Abbr‘st’,size_inv_def,all_blocks_inv_def] \\ EVAL_TAC)
+      \\ drule size_of_heap_eq_flat_size_of_heap
+      \\ disch_then (simp o single o GSYM)
+      \\ unabbrev_all_tac \\ simp[]
+      \\ simp[size_of_stack_def,size_of_stack_frame_def]
+      \\ CONV_TAC(STRIP_QUANT_CONV(LAND_CONV(SIMP_CONV std_ss [code_lookup,frame_lookup])))
+      \\ simp[]
+      \\ CONV_TAC(STRIP_QUANT_CONV(LAND_CONV EVAL))
+      \\ simp[]
+      \\ conj_tac >- EVAL_TAC
+      \\ conj_tac
+      >- (simp [sum_stack_size_def,repint_to_list_def,lookup_def,stack_consumed_def,small_num_def,
+                word_depthTheory.max_depth_def,data_to_wordTheory.AnyArith_call_tree_def]
+          \\ (fn (asm, goal) => let
+               val pat   = ``sptree$lookup _ _``
+               val terms = find_terms (can (match_term pat)) goal
+               val simps = map (PATH_CONV "lr" EVAL) terms
+              in ONCE_REWRITE_TAC simps (asm,goal) end)
+          \\ simp [frame_lookup])
+      \\ conj_tac
+      >- (simp [sum_stack_size_def,repint_to_list_def,lookup_def,stack_consumed_def,small_num_def,
+                word_depthTheory.max_depth_def,data_to_wordTheory.AnyArith_call_tree_def]
+          \\ (fn (asm, goal) => let
+               val pat   = ``sptree$lookup _ _``
+               val terms = find_terms (can (match_term pat)) goal
+               val simps = map (PATH_CONV "lr" EVAL) terms
+              in ONCE_REWRITE_TAC simps (asm,goal) end)
+          \\ simp [frame_lookup])
+      \\ conj_tac
+      >- (simp [sum_heap_size_def,repint_to_list_def,lookup_def,
+                stack_consumed_def,small_num_def,size_of_heap_def,
+                word_depthTheory.max_depth_def,data_to_wordTheory.AnyArith_call_tree_def,
+                bignum_size_def,bigest_acc_size_def,bigest_num_size_def,
+                foldadd_limit_ok_def,space_consumed_def,size_of_def]
+          \\ EVAL_TAC)
+      \\ conj_tac
+      >- ((* TODO: currently hard-coded to n=5 for no good reason *)
+          EVAL_TAC >>
+          Cases >- EVAL_TAC >>
+          ntac 4 (simp[ADD1] >>
+                  rename1 ‘n + _’ >>
+                  Cases_on ‘n’ >- EVAL_TAC >>
+                  rename1 ‘SUC n’) >>
+          simp[] >> EVAL_TAC)
+      >- simp[frame_lookup,code_lookup,foldl_body_def,
+              Int_plus_clos_body_def,Int_plus_body_def])
+  \\ simp[ to_shallow_thm, to_shallow_def, initial_state_def,foldl_body_def ]
+  \\ strip_tac
+  >- (unabbrev_all_tac \\ simp[data_safe_def])
+  \\ simp[pop_env_def,Abbr ‘st’]
+  \\ qunabbrev_tac ‘rest_call’
+  \\ strip_assign
+  \\ simp[return_def]
+  \\ eval_goalsub_tac “sptree$lookup _ _”
+  \\ simp[flush_state_def]
+  \\ simp[data_safe_def]
+end
+QED
+
+(* 23% less proof code *)
+val _ = export_theory();
